src/util/CoqWstdlib.v
@@ -1,12 +1,48 @@
 Require Import Coq.ZArith.ZArith.
-From stdpp Require Import base.
+From stdpp Require Import -(coercions)base.
 Require Export CoqInt extmap extset.
 Require CoqWeakhtbl.
 
+(*Make tagged type if the type is boolean equality*)
+Module Type EqDecTag.
+Parameter t : Type.
+Parameter tag : t -> CoqBigInt.t.
+Parameter equal : t -> t -> bool.
+Parameter equal_eq : forall x y, x = y <-> equal x y.
+End EqDecTag.
+
+(*So we don't have to prove the lemmas every time*)
+Module MakeDecTag (E: EqDecTag) <: TaggedType.
+Definition t := E.t.
+Definition tag := E.tag.
+Definition equal := E.equal.
+Lemma eq_refl : forall x, equal x x.
+Proof. intros x. apply E.equal_eq. reflexivity. Qed.
+Lemma eq_sym : forall x y, equal x y = equal y x.
+Proof.
+  intros x y.
+  destruct (equal x y) eqn : Hxy.
+  - apply E.equal_eq in Hxy. subst. symmetry. apply E.equal_eq. reflexivity.
+  - destruct (equal y x) eqn : Hyx; auto. apply E.equal_eq in Hyx; subst.
+    rewrite eq_refl in Hxy. discriminate.
+Qed.
+Lemma eq_trans: forall x y z, equal x y -> equal y z -> equal x z.
+Proof. intros x y z Heq1 Heq2. apply E.equal_eq in Heq1, Heq2. apply E.equal_eq. subst; auto.
+Qed.
+Lemma eq_compat: forall x y, equal x y -> tag x = tag y.
+Proof. intros x y Heq. apply E.equal_eq in Heq; subst; auto.
+Qed. 
+End MakeDecTag.
+
+(*TODO: can we generalize this (probably not because modules in Coq are not first class)*)
 Module BigIntTag <: TaggedType.
-Definition t := CoqBigInt.t.
-Definition tag (x: t) := x.
-Definition equal := CoqBigInt.eqb.
+  Module BigIntDecTag <: EqDecTag.
+    Definition t := CoqBigInt.t.
+    Definition tag (x: t) := x.
+    Definition equal := CoqBigInt.eqb.
+    Definition equal_eq := CoqBigInt.eqb_eq.
+  End BigIntDecTag.
+  Include MakeDecTag BigIntDecTag.
 End BigIntTag.
 
 (*A version of the Str interface where tag is implemented by
@@ -16,10 +52,15 @@ End BigIntTag.
   in future*)
 Axiom string_hash: string -> CoqBigInt.t.
 Module Str <: TaggedType.
-Definition t := string.
-Definition tag (s: string) : CoqBigInt.t := string_hash s.
-Definition equal := String.eqb.
+  Module StrDec <: EqDecTag.
+    Definition t := string.
+    Definition tag (s: string) : CoqBigInt.t := string_hash s.
+    Definition equal := String.eqb.
+    Definition equal_eq := fun x y => iff_sym (String.eqb_eq x y).
+  End StrDec.
+  Include MakeDecTag StrDec.
 End Str.
+
 Module Mstr := extmap.Make Str.
 Module Sstr := extset.MakeOfMap(Mstr).
 
@@ -29,10 +70,14 @@ Module Sstr := extset.MakeOfMap(Mstr).
     TODO maybe axiomatize hash function and implement in Coq?
     Not great more trust*)
 Module Str2 <: TaggedType.
-Definition t := string.
-Definition tag (s: string) : CoqBigInt.t :=
-  CoqBigInt.of_Z (Z.pos (str_to_pos s)).
-Definition equal := String.eqb.
+  Module Str2Dec <: EqDecTag.
+    Definition t := string.
+    Definition tag (s: string) : CoqBigInt.t :=
+      CoqBigInt.of_Z (Z.pos (str_to_pos s)).
+    Definition equal := String.eqb.
+    Definition equal_eq := fun x y => iff_sym (String.eqb_eq x y).
+  End Str2Dec.
+  Include MakeDecTag Str2Dec.
 End Str2.
 
 (*TODO: see*)
@@ -70,9 +115,13 @@ Module S := extset.MakeOfMap(M).
 End MakeMS.
 
 Module MakeTagged (X: CoqWeakhtbl.Weakey) <: TaggedType.
-Definition t := X.t.
-Definition tag x := CoqWeakhtbl.tag_hash (X.tag x).
-Definition equal := X.equal.
+  Module MakeDec <: EqDecTag.
+    Definition t := X.t.
+    Definition tag x := CoqWeakhtbl.tag_hash (X.tag x).
+    Definition equal := X.equal.
+    Definition equal_eq := X.equal_eq.
+  End MakeDec.
+  Include MakeDecTag MakeDec.
 End MakeTagged.
 
 (*Don't create a weak hashtable, but use the weakey type*)
